Add stack defthms.

stack.lisp
@@ -1,17 +1,39 @@
 (in-package "ACL2")
 
+(include-book "base")
+
 ;; The word size of the machine (and thus size of stack items) is 256-bit. The
 ;; stack has a maximum size of 1024.
 
 (defun mk-empty-stack () (list 'stack-bottom))
 
-(defun stack/validp (stack) (listp stack))
+(defun stack/has-n (stack n)
+  (and (natp n)
+       (< n (1- (length stack)))))
+
+(defun stack/validp (stack)
+  (if (stack/has-n stack 0)
+      (and (listp stack)
+           (evm-w256p (car stack))
+           (stack/validp (cdr stack)))
+      (equal stack (mk-empty-stack))))
 
 (defun stack/push (stack v)
-  (cons v stack))
+  (if (evm-w256p v)
+      (cons v stack)
+      stack))
+
+(defun stack/pop (stack)
+  (if (equal stack (mk-empty-stack))
+      stack
+      (cdr stack)))
 
 (defun stack/popn (stack n)
-  (subseq stack n nil))
+  (if (zp n)
+      stack
+      (stack/popn (stack/pop stack) (1- n))))
 
 (defun stack/n (stack n)
-  (car (stack/popn stack n)))
+  (if (stack/has-n stack n)
+      (car (stack/popn stack n))
+      0))
