base.lisp
@@ -1,0 +1,4 @@
+(in-package "ACL2")
+
+(defun evm-w256p (n)
+  (integerp n))
