exec-defthms.lisp
@@ -1,15 +1,20 @@
 (in-package "ACL2")
 
 (include-book "env")
+(include-book "env-defthms")
 (include-book "exec")
+
+;; (defthm env/exec-step-valid-io-pc
+;;     (implies (env/validp e)
+;;              (integerp (env/pc (env/step e)))))
 
 ;; (defthm env/exec-hacky-valid-io-pc-limit-step
 ;;     (implies (env/validp e)
-;;              (natp (env/pc (env/exec-hacky e 10)))))
+;;              (integerp (env/pc (env/exec-hacky e 1)))))
 
 ;; (defthm env/exec-hacky-valid-io-pc
 ;;     (implies (env/validp e)
-;;              (natp (env/pc (env/exec-hacky e n)))))
+;;              (integerp (env/pc (env/exec-hacky e n)))))
 
 ;; (defthm env/exec-hacky-valid-io
 ;;     (implies (env/validp e)
