stack-defthms.lisp
@@ -1,0 +1,15 @@
+(in-package "ACL2")
+
+(include-book "stack")
+
+(defthm stack/push-io-validp
+    (implies (stack/validp s)
+             (stack/validp (stack/push s v))))
+
+(defthm stack/pop-io-validp
+    (implies (stack/validp s)
+             (stack/validp (stack/pop s))))
+
+(defthm stack/popn-io-validp
+    (implies (stack/validp s)
+             (stack/validp (stack/popn s n))))
